code/streaming/Hacl.Streaming.Blake2s_32.fst
@@ -8,6 +8,7 @@ module Blake2s32 = Hacl.Blake2s_32
 module Common = Hacl.Streaming.Blake2.Common
 module Core = Hacl.Impl.Blake2.Core
 module F = Hacl.Streaming.Functor
+module P = Hacl.Streaming.Blake2.Params
 module I = Hacl.Streaming.Interface
 module G = FStar.Ghost
 module B = LowStar.Buffer
@@ -20,24 +21,14 @@ open FStar.HyperStack.ST
 #set-options "--fuel 0 --ifuel 0"
 
 inline_for_extraction noextract
-<<<<<<< HEAD
 let blake2s_32 =
-  Common.blake2 Spec.Blake2S Core.M32 Blake2s32.init Blake2s32.update_multi
-=======
-let blake2s_32 kk =
-  Common.blake2 Spec.Blake2S Core.M32 false kk Blake2s32.init Blake2s32.update_multi
-         Blake2s32.update_last Blake2s32.finish
-
-inline_for_extraction noextract
-let blake2s_32_params kk =
-  Common.blake2 Spec.Blake2S Core.M32 true kk Blake2s32.init_with_params Blake2s32.update_multi
->>>>>>> origin/afromher_blake
+  Common.blake2 Spec.Blake2S Core.M32 Blake2s32.init_with_params Blake2s32.update_multi
          Blake2s32.update_last Blake2s32.finish
 
 /// Type abbreviations - makes Karamel use pretty names in the generated code
 
-let block_state_t (kk: G.erased (Common.key_size_t Spec.Blake2S)) = Common.s Spec.Blake2S kk Core.M32
-let state_t (kk: G.erased (Common.key_size_t Spec.Blake2S)) =
+let block_state_t (kk: G.erased (Common.index Spec.Blake2S)) = Common.s Spec.Blake2S kk Core.M32
+let state_t (kk: G.erased (Common.index Spec.Blake2S)) =
   F.state_s blake2s_32 kk (Common.s Spec.Blake2S kk Core.M32) (Common.blake_key Spec.Blake2S kk)
 
 /// The incremental hash functions instantiations. Note that we can't write a
@@ -47,40 +38,114 @@ let state_t (kk: G.erased (Common.key_size_t Spec.Blake2S)) =
 
 inline_for_extraction noextract
 [@ (Comment "  State allocation function when there is no key")]
-let alloca_raw (kk: Common.key_size_t Spec.Blake2S): Tot _ =
+let alloca_raw (kk: Common.index Spec.Blake2S): Tot _ =
   F.alloca blake2s_32 kk (Common.s Spec.Blake2S kk Core.M32) (Common.blake_key Spec.Blake2S kk)
 
 private
-let malloc_raw (kk: Common.key_size_t Spec.Blake2S): Tot _ =
+let malloc_raw (kk: Common.index Spec.Blake2S): Tot _ =
   F.malloc blake2s_32 kk (Common.s Spec.Blake2S kk Core.M32) (Common.blake_key Spec.Blake2S kk)
 
-[@ (Comment "  State allocation function when there is a key")]
-val malloc_with_key:
-  k:LowStar.Buffer.buffer Lib.IntTypes.uint8 ->
-  kk:Common.key_size_t Spec.Blake2S { LowStar.Buffer.len k == kk } -> (
+[@ (Comment " State allocation function when there are parameters and a key. The
+length of the key k MUST match the value of the field key_length in the
+parameters. Furthermore, there is a static (not dynamically checked) requirement
+that key_length does not exceed max_key (32 for S, 64 for B).)")]
+val malloc_with_params_and_key:
+  i:G.erased (P.index Spec.Blake2S) ->
+  p:P.params Spec.Blake2S i ->
+  k:LowStar.Buffer.buffer Lib.IntTypes.uint8 { LowStar.Buffer.length k == UInt8.v (fst i) } -> (
   let open F in
   let c = blake2s_32 in
-  let i = kk in
   let t: Type0 = c.state.s i in
-  let t': Type0 = I.optional_key i c.km c.key in
-  let k: Common.stateful_key_t Spec.Blake2S kk = kk, k in
+  let t': Type0 = I.optional_key (G.reveal i) c.km c.key in
+  let k: Common.stateful_key_t Spec.Blake2S (G.reveal i) = p, k in
   r: HS.rid ->
   ST (state c i t t')
   (requires (fun h0 ->
-    c.key.invariant #i h0 k /\
+    blake2s_32.key.invariant #i h0 k /\
     HyperStack.ST.is_eternal_region r))
   (ensures (fun h0 s h1 ->
     invariant c i h1 s /\
     freeable c i h1 s /\
     seen c i h1 s == S.empty /\
-    reveal_key c i h1 s == c.key.v i h0 k /\
+    reveal_key blake2s_32 i h1 s == blake2s_32.key.v i h0 k /\
     B.(modifies loc_none h0 h1) /\
     B.fresh_loc (footprint c i h1 s) h0 h1 /\
     B.(loc_includes (loc_region_only true r) (footprint c i h1 s))))
 )
 
+let malloc_with_params_and_key i p k r =
+  let pv = P.get_params p in
+  let i = pv.Core.key_length, pv.Core.digest_length in
+  malloc_raw i (p, k) r
+
+[@ (Comment " State allocation function when there is just a custom key. All
+other parameters are set to their respective default values, meaning the output
+length is the maximum allowed output (32 for S, 64 for B).")]
+val malloc_with_key:
+  k:LowStar.Buffer.buffer Lib.IntTypes.uint8 ->
+  kk:Spec.key_length_t Spec.Blake2S { LowStar.Buffer.length k == UInt8.v kk } -> (
+  let open F in
+  let c = blake2s_32 in
+  let i: Common.index Spec.Blake2S = kk, UInt8.uint_to_t (Spec.max_output Spec.Blake2S) in
+  let t: Type0 = c.state.s i in
+  let t': Type0 = I.optional_key (G.reveal i) c.km c.key in
+  r: HS.rid ->
+  ST (state c i t t')
+  (requires (fun h0 ->
+    // This type is rather annoying to write, since we can't just copy-paste
+    // from Functor (with a few suitable names in scope).
+    B.live h0 k /\ // The other few bits required to conclude key_invariant will materialize after stack-allocating
+    HyperStack.ST.is_eternal_region r))
+  (ensures (fun h0 s h1 ->
+    invariant c i h1 s /\
+    freeable c i h1 s /\
+    seen c i h1 s == S.empty /\
+    reveal_key blake2s_32 i h1 s ==
+      ({ Spec.blake2_default_params Spec.Blake2S with Spec.key_length = kk },
+      (if fst i = 0uy then S.empty #uint8 else B.as_seq h0 (k <: B.buffer uint8))) /\
+    B.(modifies loc_none h0 h1) /\
+    B.fresh_loc (footprint c i h1 s) h0 h1 /\
+    B.(loc_includes (loc_region_only true r) (footprint c i h1 s))))
+)
+
+module ST = FStar.HyperStack.ST
+
 let malloc_with_key k kk r =
-  malloc_raw kk (kk, k) r
+  let _ = allow_inversion Spec.alg in
+  let nn = UInt8.uint_to_t (Spec.max_output Spec.Blake2S) in
+  let i: Common.index Spec.Blake2S = kk, nn in
+  let h00 = ST.get () in
+
+  let p = P.create_in Spec.Blake2S i r in
+  let h0 = ST.get () in
+  assert B.(as_seq h00 k == as_seq h0 k);
+
+  let s = malloc_with_params_and_key (G.hide i) p k r in
+  let h1 = ST.get () in
+  assert F.(freeable blake2s_32 i h1 s);
+  assert (nn == (Spec.blake2_default_params Spec.Blake2S).digest_length);
+  calc (==) {
+    F.reveal_key blake2s_32 i h1 s;
+  (==) { }
+    blake2s_32.key.v i h0 (p, k);
+  (==) { }
+    Common.key_v i h0 (p, k);
+  (==) { _ by (FStar.Tactics.trefl ()) }
+    P.v #Spec.Blake2S h0 p, (if fst i = 0uy then S.empty #Lib.IntTypes.uint8 else B.as_seq h0 (k <: B.buffer Lib.IntTypes.uint8));
+  (==) { }
+    { Spec.blake2_default_params Spec.Blake2S with Spec.key_length = kk; Spec.digest_length = nn }, (if fst i = 0uy then S.empty #Lib.IntTypes.uint8 else B.as_seq h0 (k <: B.buffer Lib.IntTypes.uint8));
+  (==) { }
+    { Spec.blake2_default_params Spec.Blake2S with Spec.key_length = kk }, (if fst i = 0uy then S.empty #Lib.IntTypes.uint8 else B.as_seq h0 (k <: B.buffer Lib.IntTypes.uint8));
+  };
+  assert (P.invariant h1 p);
+  P.invariant_loc_in_footprint h1 p;
+  assert B.(loc_disjoint (P.footprint h1 p) (F.footprint blake2s_32 i h1 s));
+  P.free p;
+  let h2 = ST.get () in
+  F.frame_invariant blake2s_32 i (P.footprint h1 p) s h1 h2;
+  F.frame_seen blake2s_32 i (P.footprint h1 p) s h1 h2;
+  assert F.(freeable blake2s_32 i h2 s);
+  s
 
 // I generally don't like skipping signatures since there's a danger that a
 // partial application generates a GTot that later on gives errors that are hard
@@ -88,8 +153,47 @@ let malloc_with_key k kk r =
 // painful to write and the refinement seems to be sufficient, so, there we go.
 [@ (Comment "  State allocation function when there is no key")]
 let malloc (r: HS.rid { HyperStack.ST.is_eternal_region r }) =
-  malloc_with_key B.null 0ul r
+  malloc_with_key B.null 0uy r
 
+private
+let index_of_state (kk: G.erased (Common.index Spec.Blake2S)): Tot _ =
+  F.index_of_state blake2s_32 kk (Common.s Spec.Blake2S kk Core.M32) (Common.blake_key Spec.Blake2S kk)
+
+private
+let reset_raw (kk: G.erased (Common.index Spec.Blake2S)): Tot _ =
+  F.reset blake2s_32 kk (Common.s Spec.Blake2S kk Core.M32) (Common.blake_key Spec.Blake2S kk)
+
+[@ (Comment " Re-initialization function. The reinitialization API is tricky --
+you MUST reuse the same original parameters for digest (output) length and key
+length.")]
+val reset_with_key_and_params: (i: G.erased (Common.index Spec.Blake2S)) -> (
+  let open F in
+  let c = blake2s_32 in
+  let t: Type0 = c.state.s (G.reveal i) in
+  let t': Type0 = I.optional_key (G.reveal i) c.km c.key in
+  state:state c (G.reveal i) t t' ->
+  p:P.params Spec.Blake2S i ->
+  k:LowStar.Buffer.buffer Lib.IntTypes.uint8 { LowStar.Buffer.length k == UInt8.v (fst i) } -> (
+  let key: Common.stateful_key_t Spec.Blake2S (G.reveal i) = (p, k) in
+  unit ->
+  Stack unit
+  (requires (fun h0 ->
+    blake2s_32.key.invariant #i h0 key /\
+    B.loc_disjoint (blake2s_32.key.footprint #i h0 key) (footprint c i h0 state) /\
+    invariant c i h0 state))
+  (ensures (fun h0 _ h1 ->
+    invariant c i h1 state /\
+    seen c i h1 state == S.empty /\
+    reveal_key c i h1 state == blake2s_32.key.v i h0 key /\
+    footprint c i h0 state == footprint c i h1 state /\
+    B.(modifies (footprint c i h0 state) h0 h1) /\
+    preserves_freeable c i state h0 h1))))
+
+let reset_with_key_and_params i s p k () =
+  let i = index_of_state i s in
+  reset_raw i s (p, k)
+
+(*
 [@ (Comment " Re-initialization function when there is a key. Note that the key
 size is not allowed to change, which is why this function does not take a key
 length -- the key has to be same key size that was originally passed to
@@ -116,21 +220,9 @@ val reset_with_key: (i: G.erased (Common.key_size_t Spec.Blake2S)) -> (
     B.(modifies (footprint c i h0 state) h0 h1) /\
     preserves_freeable c i state h0 h1))))
 
-private
-let reset_raw (kk: G.erased (Common.key_size_t Spec.Blake2S)): Tot _ =
-  F.reset blake2s_32 kk (Common.s Spec.Blake2S kk Core.M32) (Common.blake_key Spec.Blake2S kk)
-
-private
-let index_of_state (kk: G.erased (Common.key_size_t Spec.Blake2S)): Tot _ =
-  F.index_of_state blake2s_32 kk (Common.s Spec.Blake2S kk Core.M32) (Common.blake_key Spec.Blake2S kk)
-
 let reset_with_key (i: G.erased (Common.key_size_t Spec.Blake2S)) s k () =
   let kk = index_of_state i s in
   reset_raw i s (kk, k)
-
-[@ (Comment "  State allocation function when there are parameters but no key")]
-let malloc_with_params =
-  F.malloc (blake2s_32_params 0) () (Common.s Spec.Blake2S Core.M32) (Common.empty_key Spec.Blake2S)
 
 [@ (Comment "  Re-initialization function when there is no key")]
 val reset: (
@@ -158,25 +250,22 @@ val reset: (
 
 let reset s =
   reset_with_key (G.hide 0ul) s B.null ()
-
-[@ (Comment "  Re-initialization function when there are parameters but no key")]
-let reset_with_params =
-  F.reset (blake2s_32_params 0) () (Common.s Spec.Blake2S Core.M32) (Common.empty_key Spec.Blake2S)
+*)
 
 [@ (Comment "  Update function when there is no key; 0 = success, 1 = max length exceeded")]
-let update (kk: G.erased (Common.key_size_t Spec.Blake2S)): Tot _ =
+let update (kk: G.erased (Common.index Spec.Blake2S)): Tot _ =
   F.update blake2s_32 kk (Common.s Spec.Blake2S kk Core.M32) (Common.blake_key Spec.Blake2S kk)
 
 [@ (Comment "  Finish function when there is no key")]
-let digest (kk: G.erased (Common.key_size_t Spec.Blake2S)): Tot _ =
+let digest (kk: G.erased (Common.index Spec.Blake2S)): Tot _ =
   F.digest_erased blake2s_32 kk (Common.s Spec.Blake2S kk Core.M32) (Common.blake_key Spec.Blake2S kk)
 
 [@ (Comment "  Free state function when there is no key")]
-let free (kk: G.erased (Common.key_size_t Spec.Blake2S)): Tot _ =
+let free (kk: G.erased (Common.index Spec.Blake2S)): Tot _ =
   F.free blake2s_32 kk (Common.s Spec.Blake2S kk Core.M32) (Common.blake_key Spec.Blake2S kk)
 
 [@ (Comment "  Copying. The key length (or absence thereof) must match between source and destination.")]
-let copy (kk: G.erased (Common.key_size_t Spec.Blake2S)): Tot _ =
+let copy (kk: G.erased (Common.index Spec.Blake2S)): Tot _ =
   F.copy blake2s_32 kk (Common.s Spec.Blake2S kk Core.M32) (Common.blake_key Spec.Blake2S kk)
 
 (* The one-shot hash *)
@@ -190,3 +279,6 @@ let copy (kk: G.erased (Common.key_size_t Spec.Blake2S)): Tot _ =
 @param key_len Length of the key. Can be 0."]
 let hash_with_key : Impl.blake2_st Spec.Blake2S Core.M32 =
   Impl.blake2 #Spec.Blake2S #Core.M32 Blake2s32.init Blake2s32.update Blake2s32.finish
+
+let hash_with_key_and_paramas : Impl.blake2_with_params_st Spec.Blake2S Core.M32 =
+  Impl.blake2_with_params #Spec.Blake2S #Core.M32 Blake2s32.init_with_params Blake2s32.update Blake2s32.finish
